Exercise 7.2

ch7/IMP.thy
@@ -82,8 +82,15 @@ WhileTrue: "
   \<Longrightarrow> (WHILE b DO c,s1) \<Rightarrow> s3
 "
 
-inductive big_step_induct :: "com \<Rightarrow> state \<Rightarrow> state \<Rightarrow> bool" where
-"(c,s) \<Rightarrow> t \<Longrightarrow> big_step_induct c s t"
+(* Big step tweaks to simplify usage as found in
+   the implementation included in the Isabelle source *)
+declare big_step.intros [intro]
+lemmas big_step_induct = big_step.induct[split_format(complete)]
+inductive_cases SkipE[elim!]: "(SKIP,s) \<Rightarrow> t"
+inductive_cases AssignE[elim!]: "(x ::= c,s) \<Rightarrow> t"
+inductive_cases SeqE[elim!]: "(c1 ;; c2,s) \<Rightarrow> t"
+inductive_cases IfE[elim!]: "(IF b THEN c1 ELSE c2,s) \<Rightarrow> t"
+inductive_cases WhileE[elim]: "(WHILE b DO c,s) \<Rightarrow> t"
 
 (* Small-step semantic rules from 7.3 *)
 inductive small_step :: "com \<times> state \<Rightarrow> com \<times> state \<Rightarrow> bool"
@@ -94,6 +101,178 @@ Seq2: "(c1,s) \<rightarrow> (c1',s') \<Longrightarrow> (c1;;c2,s) \<rightarrow> 
 IfTrue: "bval b s \<Longrightarrow> (IF b THEN c1 ELSE c2,s) \<rightarrow> (c1,s)" |
 IfFalse: "\<not>bval b s \<Longrightarrow> (IF b THEN c1 ELSE c2,s) \<rightarrow> (c2,s)" |
 While: "(WHILE b DO c,s) \<rightarrow> (IF b THEN c;;WHILE b DO c ELSE SKIP,s)"
+
+
+(* Semantic helpers *)
+
+(* Rule inversion equivalence lemmas from 7.2.3 *)
+lemma skip_state_equiv:
+  "(SKIP,s) \<Rightarrow> t \<longleftrightarrow> t = s" (is "?LHS \<longleftrightarrow> ?RHS")
+proof
+  assume "?LHS"
+  thus "?RHS" by cases
+next
+  assume "?RHS"
+  thus "?LHS" by (simp add: Skip)
+qed
+
+lemma assign_state:
+  "(x ::= a,s) \<Rightarrow> t \<longleftrightarrow> t = s(x := aval a s)"
+  (is "?LHS \<longleftrightarrow> ?RHS")
+proof
+  assume "?LHS"
+  thus "?RHS" by cases
+next
+  assume "?RHS"
+  thus "?LHS" using big_step.Assign by blast
+qed
+
+lemma inter_seq:
+  "(c1 ;; c2,s1) \<Rightarrow> s3
+    \<longleftrightarrow> (\<exists>s2. ((c1,s1) \<Rightarrow> s2 \<and> (c2,s2) \<Rightarrow> s3))"
+  (is "?LHS \<longleftrightarrow> ?RHS")
+proof
+  assume "?LHS"
+  thus "?RHS"
+  proof cases
+    case Seq thus ?thesis by auto
+  qed
+next
+  assume "?RHS"
+  thus "?LHS" using Seq by blast
+qed
+
+lemma while_split:
+  "(WHILE b DO c,s) \<Rightarrow> t
+    \<longleftrightarrow> (
+      \<not> bval b s \<and> t = s
+      \<or> bval b s
+        \<and> (\<exists>s'. (c,s) \<Rightarrow> s'
+            \<and> (WHILE b DO c,s') \<Rightarrow> t))"
+  (is "?LHS \<longleftrightarrow> ?RHS")
+proof
+  assume "?LHS"
+  thus "?RHS"
+  proof cases
+    case WhileFalse
+    thus ?thesis by auto
+  next
+    case WhileTrue
+    thus ?thesis by auto
+  qed
+next
+  assume "?RHS"
+  thus "?LHS"
+    using WhileFalse WhileTrue by blast
+qed
+
+(* Associativity of Seq from 7.2.3 *)
+lemma seq_assoc:
+  "((c1 ;; c2) ;; c3,s) \<Rightarrow> s'
+   \<longleftrightarrow> (c1 ;; (c2 ;; c3),s) \<Rightarrow> s'"
+  (is "?LHS \<longleftrightarrow> ?RHS")
+proof
+  assume "?LHS"
+  then obtain s1 s2 where
+    "(c1,s) \<Rightarrow> s1" and
+    "(c2,s1) \<Rightarrow> s2" and
+    "(c3,s2) \<Rightarrow> s'"
+    using inter_seq by blast
+  thus "?RHS" by (simp add: Seq)
+next
+  assume "?RHS"
+  then obtain s1 s2 where
+    "(c1,s) \<Rightarrow> s1" and
+    "(c2,s1) \<Rightarrow> s2" and
+    "(c3,s2) \<Rightarrow> s'"
+    using inter_seq by blast
+  thus "?LHS"
+    using Seq by blast
+qed
+
+(* Big-step equivalence from 7.2.4 *)
+abbreviation equiv_c :: "com \<Rightarrow> com \<Rightarrow> bool"
+  (infix "\<sim>" 50) where
+"c \<sim> c' \<equiv> (\<forall>s. \<forall>t. ((c,s) \<Rightarrow> t = (c',s) \<Rightarrow> t))"
+
+(* While is equivalent to a single unfold of itself *)
+lemma while_is_unfolded_while:
+  "(WHILE b DO c)
+    \<sim> (IF b THEN c ;; WHILE b DO c ELSE SKIP)"
+  (is "?LHS \<sim> ?RHS")
+proof -
+  have "(?RHS,s) \<Rightarrow> t" if assm: "(?LHS,s) \<Rightarrow> t" for s t
+  proof -
+    from assm show ?thesis
+    proof cases
+      case WhileTrue
+      from this `bval b s` `(?LHS,s) \<Rightarrow> t`
+      obtain s'
+        where "(c,s) \<Rightarrow> s'" and "(?LHS,s') \<Rightarrow> t"
+        by blast
+      hence "(c ;; ?LHS,s) \<Rightarrow> t" by (rule Seq)
+      thus ?thesis using `bval b s` by auto
+    next
+      case WhileFalse
+      thus ?thesis by auto
+    qed
+  qed
+  moreover
+  have "(?LHS,s) \<Rightarrow> t" if assm: "(?RHS,s) \<Rightarrow> t" for s t
+  proof -
+    from assm show ?thesis
+    proof cases
+      case IfTrue
+      from this inter_seq obtain s'
+        where "(c,s) \<Rightarrow> s'" and "(?LHS,s') \<Rightarrow> t"
+        by blast
+      thus ?thesis using IfTrue by blast
+    next
+      case IfFalse
+      hence "s = t" using skip_state_equiv by simp
+      thus ?thesis using IfFalse by blast
+    qed
+  qed
+  ultimately
+  show ?thesis by blast
+qed
+
+(* The previous proof is likely clearer,
+   but all that inductive_case stuff allows
+   full auto here *)
+lemma "(WHILE b DO c) \<sim> (IF b THEN c ;; WHILE b DO c ELSE SKIP)"
+  by blast
+
+(* A command in both if clauses is equivalent
+   to the command *)
+lemma if_both_com_is_com:
+  "(IF b THEN c ELSE c) \<sim> c"
+  by blast
+
+(* Big-step equivalence is an equivalence relation *)
+theorem refl_equiv_c: "c \<sim> c" by auto
+theorem sym_equiv_c: "c1 \<sim> c2 \<Longrightarrow> c2 \<sim> c1" by auto
+theorem trans_equiv_c: "c1 \<sim> c2 \<and> c2 \<sim> c3 \<Longrightarrow> c1 \<sim> c3"
+  by auto
+
+(* IMP is deterministic from 7.2.5 *)
+theorem imp_deterministic:
+  "(c,s) \<Rightarrow> t \<Longrightarrow> (c,s) \<Rightarrow> t' \<Longrightarrow> t' = t"
+proof (induction arbitrary: t' rule: big_step.induct)
+  fix b c s s1 t t'
+  assume "bval b s"
+    and "(c,s) \<Rightarrow> s1"
+    and "(WHILE b DO c,s1) \<Rightarrow> t"
+  assume IHc: "\<And>t'. (c,s) \<Rightarrow> t' \<Longrightarrow> t' = s1"
+  assume IHw: "\<And>t'. (WHILE b DO c,s1) \<Rightarrow> t' \<Longrightarrow> t' = t"
+  assume "(WHILE b DO c,s) \<Rightarrow> t'"
+  with `bval b s` obtain s1' where
+    c: "(c,s) \<Rightarrow> s1'" and
+    w: "(WHILE b DO c,s1') \<Rightarrow> t'"
+    by auto
+  from c IHc have "s1' = s1" by blast
+  with w IHw show "t' = t" by blast
+qed blast+
 
 (* Reflexive transitive closure from 4.5.2 *)
 (* Needed for closure of small-step semantic *)
