ch7/Exercise2.thy
@@ -1,0 +1,37 @@
+theory Exercise2
+  imports IMP
+begin
+
+(* NOTE: Just as with assigned_oe from Exercise 1,
+   skip_ua is an inaccurate approximation (in this case,
+   an underapproximation of SKIP-equivalent commands, or
+   an overapproximation of non-SKIP-equivalent
+   commands. Also of note, given the command WHILE g
+   DO c, if c is equivalent to SKIP then the while loop
+   would never terminate (which we could reasonably say
+   is not equivalent behavior to SKIP). Since we have
+   already chosen not to explore satisfiability of guards
+   with skip_ua, we will just say the WHILE g DO c form
+   is not equivalent to SKIP. *)
+fun skip_ua :: "com \<Rightarrow> bool" where
+skip: "skip_ua (SKIP) = True" |
+assign: "skip_ua (x ::= a) = False" |
+seq: "skip_ua (a ;; b) = ((skip_ua a) \<and> (skip_ua b))" |
+ifthen: "skip_ua (IF g THEN a ELSE b)
+  = ((skip_ua a) \<and> (skip_ua b))" |
+whiledo: "skip_ua (WHILE g DO a) = False"
+
+theorem skip_ua_impl_equiv: "skip_ua c \<Longrightarrow> c \<sim> SKIP"
+proof (induction c)
+  case (Seq c1 c2)
+  hence "c1 \<sim> SKIP" and "c2 \<sim> SKIP" by simp_all
+  hence "(c1 ;; c2) \<sim> (SKIP ;; SKIP)" by blast
+  thus "(c1 ;; c2) \<sim> SKIP" by auto
+next
+  case (If b c1 c2)
+  hence "c1 \<sim> SKIP" and "c2 \<sim> SKIP" by simp_all
+  thus "(IF b THEN c1 ELSE c2) \<sim> SKIP"
+    by blast
+qed auto
+
+end
